ironfleet/src/Dafny/Distributed/Services/Lock/TrueMain.i.dfy
@@ -1,0 +1,65 @@
+include "Main.i.dfy"
+include "../../Concur/QuantizedSystem.s.dfy"
+
+module TrueMain_i {
+    import opened Main_i
+    import opened QuantizedSystem_s 
+
+    function LeaseSpecIoFilter(config:ConcreteConfiguration) : IoPredicate
+    {
+        (io:IoOp) -> exists epoch :: io.LIoOpReceive?
+                                  && io.r.msg == MarshallLockMsg(epoch) 
+                                  && io.r.src in config
+                                  && io.r.dst !in config
+    }
+
+    ghost method GenerateQbToDbMapping(config:ConcreteConfiguration, qb:seq<QS_State>, db:seq<DS_State>, external_io:IoPred) returns (cm:seq<int>)
+        requires |qb| > 0;
+        requires QS_Init(qb[0], config);
+        requires forall i {:trigger QS_Next(qb[i], qb[i+1])} :: 0 <= i < |qb| - 1 ==> QS_Next(qb[i], qb[i+1]);
+        requires  |db'| > 0;
+        requires  DS_Init(db'[0], config);
+        requires  forall i {:trigger DS_Next(db'[i], db'[i+1])} :: 0 <= i < |db'| - 1 ==> DS_Next(db'[i], db'[i+1]);
+        requires ProjectExternalIO(qb, external_io(config)) == ProjectDsExternalIO(db', external_io(config));
+        ensures  |qb| == |cm|;     
+        ensures  cm[0] == 0;                                            // Beginnings match
+        ensures  forall i :: 0 <= i < |cm| && IsFixedStep(qb[i], external_io(config)) ==> 0 <= cm[i] < |db'|;       // Mappings we care about are in bounds
+        ensures  forall i, j :: 0 <= i < j < |cm| && IsFixedStep(qb[i], external_io(config)) && IsFixedStep(qb[j], external_io(config)) ==> cm[i] <= cm[j];    // Mapping is monotonic for the external IOs
+    {
+        if |qb| == 1 {
+            
+        } else {
+
+        }
+
+    }
+
+    lemma UltimateRefinementProof(config:ConcreteConfiguration, qb:seq<QS_State>) returns (sb:seq<ServiceState>, cm:seq<int>)
+        requires |qb| > 0;
+        requires QS_Init(qb[0], config);
+        requires forall i {:trigger QS_Next(qb[i], qb[i+1])} :: 0 <= i < |qb| - 1 ==> QS_Next(qb[i], qb[i+1]);
+        requires var trace:StepTrace := ComputeStepTrace(qb);
+                 forall host :: host in qb[0].servers ==> 
+                     exists io_partition:seq<IoTrace>, behavior:seq<HostState> :: 
+                         SeqCat(io_partition) == ProjectStepTraceToHostIos(trace, host) 
+                      && |io_partition| == |behavior| - 1
+                      && (forall i :: 0 <= i < |io_partition| ==> HostNext(behavior[i], behavior[i+1], io_partition[i])); 
+        ensures  |qb| == |cm|;
+        ensures  cm[0] == 0;                                            // Beginnings match
+        ensures  forall i :: 0 <= i < |cm| ==> 0 <= cm[i] < |sb|;       // Mappings are in bounds
+        ensures  forall i {:trigger cm[i], cm[i+1]} :: 0 <= i < |cm| - 1 ==> cm[i] <= cm[i+1];    // Mapping is monotonic
+        ensures  Service_Init(sb[0], Collections__Maps2_s.mapdomain(qb[0].servers));
+        ensures  forall i {:trigger Service_Next(sb[i], sb[i+1])} :: 0 <= i < |sb| - 1 ==> Service_Next(sb[i], sb[i+1]);
+        ensures  forall i :: 0 <= i < |qb| ==> Service_Correspondence(qb[i].environment.nextStep, sb[cm[i]]);
+    {
+        var qb', db', cm_step1 := BryansProof(config, qb, LeaseSpecIoFilter); 
+
+        var cm_step2;
+        sb, cm_step2 := RefinementProof(config, db');
+
+
+        assume false;
+
+
+    }
+}
